@base <https://gont.ch/> .
@prefix rdf: <http://www.w3.org/1999/02/22-rdf-syntax-ns#> .
@prefix rdfs: <http://www.w3.org/2000/01/rdf-schema#> .
@prefix owl: <http://www.w3.org/2002/07/owl#> .
@prefix dcterms: <http://purl.org/dc/terms/> .
@prefix xsd: <http://www.w3.org/2001/XMLSchema#> .
@prefix skos: <http://www.w3.org/2004/02/skos/core#> .
@prefix schema: <http://schema.org> .

# id, range integer
# name: skos-label
# synonyme: skos alt-label
# aktion p und d übernehmen, mit klasse Aktion als object
# rechtliche Grundlage: legalBasisDescription (range literal), legalBasis (range: Gesetz/verorrdnung - "Norm"/ lkif:"Legal_Source", URI? web URI oder data)

<GovernmentService> a rdfs:Class, owl:Class;
   skos:prefLabel "Government Service"@en;
   skos:prefLabel "Behörden Leistung"@de;
   skos:altLabel "Öffentliche Leistung"@de;
   rdfs:comment "TODO: check relation to schema:Service and GovernmentService";
   rdfs:comment "Defined as 'Leistung' in eCH-177 vocabulary, specified in ECH-73.".


# Service catalog related classes and properties

<ServiceCatalogEntry> a rdfs:Class, owl:Class;
   skos:prefLabel "Service Cat-alog Entry"@en;
   skos:prefLabel "Eintrag Leistungsinventar"@de;
   skos:definition "Eine Leistung gemäss eCH-0070";
   rdfs:subClassOf [
      a owl:Restrictions;
      owl:onProperty dcterms:title;
      owl:minCardinality 1
   ].


<serviceCatalogEntry> a rdf:Property ;
    skos:prefLabel "Service Catalog Entry"@en ;
    skos:prefLabel "Eintrag im Leistungskatalog"@de ;
    skos:definition "Points to the kind of service of the subject pointing to a Service Catalog Entry"@en;
    rdfs:domain <GovernmentService> ;
    rdfs:range <ServiceCatalogEntry> .


<recommendedAdditionalService> a rdf:Property ;
    skos:prefLabel "Recommended Additional Service"@en ;
    skos:prefLabel "Empfohlene Zusatzdiensleistung"@de ;
    skos:definition "Points to a recommended additional service related to the subject."@en;
    rdfs:domain <GovernmentService> ;
    rdfs:range <GovernmentService> .

<serviceProvider> a rdf:Property ;
    skos:prefLabel "Service Provider"@en ;
    skos:prefLabel "Leistungerbringer"@de ;
    skos:prefLabel "Furnitur da prestaziuns"@rm ;
    skos:definition "Points to the provider of the subject, usually a GovernmentOrganization"@de;
    rdfs:domain <GovernmentService> ;
    rdfs:range schema:Organization .

<serviceOutput> a rdf:Property ;
    skos:prefLabel "Service Output"@en ;
    skos:prefLabel "Output der Dienstleistung"@de ;
    skos:definition "Point to an output (normally identified by an IRI) that will be returned to the entity procuring the service."@de;
    rdfs:domain <GovernmentService>.

<restriction> a rdf:Property ;
    skos:prefLabel "Restriction"@en ;
    skos:prefLabel "Einschränkung"@de ;
    skos:definition "Point to a restriction on the availability of the subject."@de;
    rdfs:domain <GovernmentService>;
    rdfs:range <Restriction>.

<actionD> a rdf:Property ;
    skos:prefLabel "Action (distribution)"@en ;
    skos:prefLabel "Aktion (Vertrieb)"@de ;
    skos:definition "Points to the verb denoting the action of procuring the service."@de;
    rdfs:domain <ServiceCatalogEntry> ;
    rdfs:range xsd:string .

<actionP> a rdf:Property ;
    skos:prefLabel "Action (production)"@en ;
    skos:prefLabel "Aktion (Produktion)"@de ;
    skos:definition "Points to the verb denoting the action of rendering the service."@de;
    rdfs:domain <ServiceCatalogEntry> ;
    rdfs:range xsd:string .

<serviceResultDescription> a rdf:Property ; #And what name for the result document/product IRI? "product"? "serviceProduct", "resultDocument"- or rename this to serviceResultDescription?
    skos:prefLabel "Service Result"@en ;
    skos:prefLabel "Ergebnis der Leistung"@de ;
    skos:definition "Points to a literal describing the results of the service, e.g. 'Decision on construction permit'."@de;
    rdfs:domain <ServiceCatalogEntry> ;
    rdfs:range xsd:string .

<serviceDescription> a rdf:Property ;
    skos:prefLabel "Service Description"@en ;
    skos:prefLabel "Beschreibung der Leistung"@de ;
    skos:definition "Points to a literal providing a short description of the service."@de;
    rdfs:domain [ owl:unionOf ( <GovernmentService> <ServiceCatalogEntry> ) ];
    rdfs:range xsd:string .

<descriptor> a rdf:Property ;
    skos:prefLabel "Descriptor"@en ;
    skos:prefLabel "Deskriptor"@de ;
    skos:definition "Points to a a term describing the subject."@de;
    rdfs:domain <ServiceCatalogEntry> ; #probably more generic
    rdfs:range xsd:string.

<abbreviation> a rdf:Property ;
    skos:prefLabel "Abbreviation"@en ;
    skos:prefLabel "Kürzel"@de ;
    skos:altLabel "Kurzform"@de;
    skos:definition "Points to the (official) abbreviated name of the subject."@de;
    rdfs:range xsd:string;
    rdfs:comment "eCH-0186 introduces 'Behördenkürzel', generalized here".

<territorialCommunityAssociation> a rdf:Property ;
    skos:prefLabel "Association with Territorial Community"@en ;
    skos:prefLabel "Zugehörigkeit zu Gebietskörperschaft"@en ;
    skos:definition "Points to the territotial community (e.g. commune or canton) to which the subject is associated. In most cases a government organization is associated to only one territrial community, but there are exceptions, e.g. 'Lufthygieneamt beider Basel'.";
    rdfs:range <TerritorialCommunity> ;
    rdfs:domain <GovernmentOrganization>.


<fee> a rdf:Property;
    skos:prefLabel "Fee"@en;
    skos:prefLabel "Gebühr"@de;
    skos:definition "Eine Abgabe, die für das Erbringen einer Leistung oder für die mit der Leistung verbundene Nutzniessung eines Geschäftsobjekts erhoben wird ."@de;
    rdfs:comment "Defined in eCH-177 vocabulary";
    rdfs:domain <GovernmentService> ;
    rdfs:range xsd:decimal .


<Address> a rdfs:Class, owl:Class;
    skos:prefLabel "Address"@en;
    skos:prefLabel "Adresse"@de;
    skos:definition "Kanalspezifische Identifikation eines Absenders oder Empfängers bei der Übermittlung von Informationen"@de;
    rdfs:comment "Defined in eCH-177 vocabulary, specified in eCH-0046".

<Function> a rdfs:Class, owl:Class;
    skos:prefLabel "Function"@en;
    skos:prefLabel "Aufgabe"@de;
    skos:altLabel "Öffentliche Funktion"@de;
    skos:altLabel "Verwaltungsaufgabe"@de;
    skos:altLabel "Behördliche Funktion"@de;
    skos:definition "Eine durch gesetzliche Vorschrift einer Behörde übertragene, mittels Leistungen erfüllte staatliche Funktion."@de;
    rdfs:comment "Defined in eCH-177 vocabulary".

<GovernmentOrganization> a rdfs:Class, owl:Class;
    skos:prefLabel "GovernmentOrganization"@en;
    skos:prefLabel "Behörde"@de;
    skos:definition "Organ des Staates (Bund, Kanton) oder eines selbständigen Verwaltungs­trägers (Bezirk, Gemeinde), das Aufgaben der öffentlichen Verwaltung des Staates oder Verwaltungsträgers wahrnimmt und diesen im zugewiesenen Zuständig­keitsbereich nach Aussen vertritt."@de;
    rdfs:subClassOf schema:GovernmentOrganization;
    rdfs:comment "Defined in eCH-177 vocabulary, specified in eCH-0186. IRI of the resource is the Agency Identification ('Behördenidentifikator') requred by eCH-0186.";
    rdfs:subClassOf [
       a owl:Restrictions;
       owl:onProperty schema:name;
       owl:minCardinality 1
    ].

<Restriction> a rdfs:Class, owl:Class;
    skos:prefLabel "Restriction"@en;
    skos:prefLabel "Einschränkung"@de;
    skos:definition "A restriction of availability. An instance of Restriction is associated to the restricted service via the property 'restriction'."@en.

<DelayRestriction> a rdfs:Class, owl:Class;
    rdfs:subClassOf <Restriction>;
    skos:definition "Defines a restriction to a delay expressed as relative to a key date"@en.

<delayStart> a rdf:Property;
    skos:prefLabel "Start of delay"@en;
    skos:prefLabel "Beginn der Frist"@de;
    skos:definition "Der beginn der fist relativ zum stichtag."@de;
    rdfs:domain <DelayRestriction> ;
    rdfs:range xsd:duration .

<delayEnd> a rdf:Property;
    skos:prefLabel "End of delay"@en;
    skos:prefLabel "Ende der Frist"@de;
    skos:definition "Der beginn der fist relativ zum stichtag."@de;
    rdfs:domain <DelayRestriction> ;
    rdfs:range xsd:duration .

<AgeRestriction> a rdfs:Class, owl:Class;
    rdfs:subClassOf <Restriction>;
    skos:definition "Defines a restriction on the age of the person procuring a service"@en.

<minAge> a rdf:Property;
    skos:prefLabel "Minimum Age"@en;
    skos:prefLabel "Mindestalter"@de;
    skos:definition "Das Mindestalter in Jahre"@de;
    rdfs:domain <AgeRestriction> ;
    rdfs:range xsd:int .

<maxAge> a rdf:Property;
    skos:prefLabel "Maximum Age"@en;
    skos:prefLabel "Höchstalter"@de;
    skos:definition "Das Höchstalter in Jahre"@de;
    rdfs:domain <AgeRestriction> ;
    rdfs:range xsd:int .